\begin{prop}
If $G = G_1 \vee G_2$, then $\Jac(G)=\Jac(G_1) \oplus \Jac(G_2)$.
\end{prop}
\begin{proof}
Fix two graph isomorphisms $\psi_1, \psi_2$ that map $G_1, G_2$ into their corresponding subgraphs of $G$ (respectively). Define the map $\iota_1: \Div^0(G_1) \hookrightarrow \Div^0(G)$ by
\[
\iota_1 \left(\sum_{v \in V(G_1)}a_v v \right)= \sum_{v \in V(G_1)}a_{v} \psi(v),
\]
and define $\iota_2 : \Div^0(G_2) \hookrightarrow \Div^0(G)$ analogously. 

Now let $D, E \in \Div^0(G)$ be given; we can uniquely write
\[
D = D_1 + D_2 \quad \text{and} \quad E = E_1 + E_2,
\]
where $D_1, E_1 \in \im(\iota_1)$ and $D_2, E_2 \in \im(\iota_2)$. It suffices to show that
\[
\pair{D}{E}_G = \pair{\iota_1^{-1}(D_1)}{\iota_1^{-1}(E_1)}_{G_1} + \pair{\iota_2^{-1}(D_2)}{\iota_2^{-1}(E_2)}_{G_2}.
\]
Let $m = |\Jac(G)|$, so $m \cdot \iota_1^{-1}(E_1) \in \im(\Delta_1)$ and $m \cdot \iota_2^{-1}(E_2) \in \im(\Delta_2)$. Now choose $f_1 \in \Delta_1^{-1} (m \cdot \iota_1^{-1}(E_1))$ and $f_2 \in \Delta_2^{-1} (m \cdot \iota_2^{-1}(E_2))$ such that $f_1(\psi_1^{-1}(v_0)) = f_2(\psi_2^{-1}(v_0)) = 0$. We lift these to functions $\widehat{f_1}, \widehat{f_2} \in \mathcal{M}(G)$ be defining
\[
\widehat{f_1}(v) =
\begin{cases}
f_1(\psi_1^{-1}(v)) & \text{if $v \in V(\im(\psi_1))$} \\
0 & \text{if $v \notin V(\im(\psi_1))$},
\end{cases}
\]
and analogously for $\widehat{f_2}$.

Now we claim that $\widehat{f_1} \in \Delta^{-1}(mE_1)$ and $\widehat{f_2} \in \Delta^{-1}(mE_2)$. We prove this just for $\widehat{f_1}$, since the proof for $\widehat{f_2}$ is analogous. First, note that $\Delta(\widehat{f_1})(v)=0=mE_1(v)$ for all $v \notin V(\im(\psi_1))$. Then note that $\Delta_1(f_1)(u) = m \cdot \iota_1^{-1}(E_1)(u)$ for all $u \in V(G_1)$, so by taking $\psi_1(u)=v$, we get
\[
\Delta_1(f_1)(u) = \Delta_1(f_1)(\psi_1^{-1}(v)) = m \cdot \iota_1^{-1}(E_1)(\psi_1^{-1}(v)) = mE_1(v)
\]
for all $u \in V(G_1)$. Now we have
\begin{align*}
\Delta_1(f_1)(u) &= \ord_{u}(f_1) = \sum_{\{u,w\} \in E(G_1)} f_1(u) - f_1(w) \\
&= \sum_{\{\psi_1(u),\psi_1(w)\} \in E(G)} \widehat{f_1}(\psi_1(u)) - \widehat{f_1}(\psi_1(w)) = \ord_{\psi_1(u)}(\widehat{f_1}) = \Delta(\widehat{f_1})(v),
\end{align*}
so we deduce that $\Delta(\widehat{f_1})(v)=mE_1(v)$ for all $v\in V(\im(\psi_1))$ as well, and hence $\widehat{f_1}\in\Delta^{-1}(mE_1)$, as desired.

Now by the definition of the monodromy pairing in [CITE SHOKRIEH],
\begin{align*}
\pair{D_1}{E_1}_G &= \frac{1}{m} \sum_{v \in V(G)} D_1(v) \widehat{f_1}(v) = \frac{1}{m} \sum_{v \in V(\psi_1(G_1))} D_1(v) \widehat{f_1}(v) \\ 
&= \frac{1}{m} \sum_{u \in V(G_1)} D_1(\psi_1(u)) \widehat{f_1}(\psi_1(u)) = \frac{1}{m} \sum_{u\in V(G_1)} \iota_1^{-1}(D_1)(u)f_1(u) \\
&= \pair{\iota_1^{-1}(D_1)}{\iota_1^{-1}(E_1)}_{G_1}.
\end{align*}
An analogous argument shows that $\pair{D_2}{E_2}_G = \pair{\iota_1^{-1}(D_2)}{\iota_1^{-1}(E_2)}_{G_2}$. Further,
\[
\pair{D_1}{E_2}_G = \frac{1}{m} \sum_{v \in V(G)} D_1(v) \widehat{f_2}(v) = 0,
\]
since $\widehat{f_2}(v)=0$ when $v\in V(\im(\psi_1))$ and $D_1(v)=0$ when $v\notin V(\im(\psi_1))$. An identical argument shows that $\pair{D_2}{E_1}_G = 0$. Therefore, by bilinearity,
\begin{align*}
\pair{D}{E}_G &= \pair{D_1}{E_1} + \pair{D_1}{E_2} + \pair{D_2}{E_1} + \pair{D_2}{E_2} \\
&= \pair{\iota_1^{-1}(D_1)}{\iota_1^{-1}(E_1)}_{G_1} + \pair{\iota_2^{-1}(D_2)}{\iota_2^{-1}(E_2)}_{G_2},
\end{align*}
as desired.
\end{proof}